theories/interp_instantiate_sound.v
@@ -6,28 +6,10 @@ From mathcomp Require Import ssreflect ssrbool ssrnat eqtype seq.
 From Wasm Require Import interpreter_ctx instantiation_func instantiation_properties type_checker_reflects_typing.
 From Coq Require Import Program.
 
-Lemma Forall2_all2_impl {X Y: Type} (f: X -> Y -> bool) (fprop: X -> Y -> Prop) l1 l2:
-  (forall x y, f x y = true -> fprop x y) ->
-  all2 f l1 l2 ->
-  List.Forall2 fprop l1 l2.
-Proof.
-  move: l2.
-  induction l1; destruct l2 => //=; move => Himpl Hall.
-  move/andP in Hall; destruct Hall as [Hf Hall].
-  constructor; last by apply IHl1.
-  by apply Himpl.
-Qed.
-
 Section Host.
 
 Context `{ho: host}.
   
-Variable host_application_impl : host_state -> store_record -> function_type -> host_function -> seq value ->
-                       (host_state * option (store_record * result)).
-
-Hypothesis host_application_impl_correct :
-  (forall hs s ft hf vs hs' hres, (host_application_impl hs s ft hf vs = (hs', hres)) -> host_application hs s ft hf vs hs' hres).
-
 Lemma module_type_checker_sound: forall m t_imps t_exps,
   module_type_checker m = Some (t_imps, t_exps) ->
   module_typing m t_imps t_exps.
@@ -212,20 +194,6 @@ Qed.
    context with only the imported globals added. *)
 Lemma module_typecheck_glob_aux: forall m t_imps t_exps,
     module_type_checker m = Some (t_imps, t_exps) ->
- (*   let c' :=
-      {|
-        tc_types := [::];
-        tc_funcs := [::];
-        tc_tables := [::];
-        tc_mems := [::];
-        tc_globals := ext_t_globs t_imps;
-        tc_elems := [::];
-        tc_datas := [::];
-        tc_locals := [::];
-        tc_labels := [::];
-        tc_return := None;
-        tc_refs := [::]
-      |} in*)
     exists c, all (module_global_type_checker c) m.(mod_globals).
 Proof.
   move => m t_imps t_exps.
@@ -249,111 +217,19 @@ Proof.
   simpl in *.
   by eexists; eauto.
 Qed.
-
-Lemma module_typecheck_data_aux: forall m t_imps t_exps,
-    module_type_checker m = Some (t_imps, t_exps) ->
-    exists c, all (module_data_type_checker c) m.(mod_datas).
-Proof.
-  move => m t_imps t_exps.
-  unfold module_type_checker.
-  move => Hmodcheck.
-  destruct m.
-  remove_bools_options.
-  simpl in *.
-  by eexists; eauto.
-Qed.
-
-(* A slightly difficult proof due to having to prove additional properties of the certified interpreter.
-   Note that the reduction property can be obtained trivially, but any additional proofs on top are difficult.
-   In this case, we're 'misusing' the interpreter (running with the technically 'wrong' store) and proving that 
-   the result is still correct regardless -- therefore the predictable trouble here. *)
-Lemma interp_get_v_sglob: forall hs s f j k,
-    interp_get_v host_application_impl host_application_impl_correct hs s f [::BI_global_get j] = Some k ->
-    sglob_val s f.(f_inst) j = Some k.
-(*
-Proof.
-  move => hs s f j k Heval.
-  unfold interp_get_v, run_multi_step_raw, interpreter_ctx.run_multi_step_raw in Heval.
-  destruct (run_v_init_with_frame s f 1 _) eqn:Hrvi => //.
-  cbn in Hrvi.
-  injection Hrvi as <-.
-  destruct (run_multi_step_ctx _ _) as [ | vs] eqn:Hrmsc => //.
-  do 2 destruct vs => //.
-  injection Heval as ->.
-  unfold run_multi_step_ctx in Hrmsc.
-
-  destruct (run_one_step_ctx _ _ _) as [? cfg Hred | hs' s' rvs <- <- Heqvs | hs' s' rvs n f' <- <- Heqvs | |] eqn:Hrosc => //.
-  { destruct cfg as [[[hs0 ccs] sc] e].
-    simpl in Hred.
-    simpl in Hrosc.
-    move: Hrosc.
-    (* Coq's destruct has no clue on how to generalize the terms correctly. *)
-    move: (@Logic.eq_refl (option value) (sglob_val s f.(f_inst) j)).
-    case: {2 3} (sglob_val s f.(f_inst) j) => /=.
-
-    - move => v Hsglob Heval.
-      inversion Heval; subst; clear Heval.
-      simpl in Hrmsc.
-      inversion Hrmsc; subst.
-      exact Hsglob.
-      
-    - move => ? Hcontra.
-      by inversion Hcontra.
-  }
-  { inversion Hrmsc; subst.
-    simpl in Heqvs.
-    injection Heqvs as Heqv.
-    symmetry in Heqv.
-    by rewrite ve_inv in Heqv.
-  }
-  { inversion Hrmsc; subst.
-    simpl in Heqvs.
-    inversion Heqvs; subst.
-    symmetry in H2.
-    by rewrite ve_inv in H2.
-  }
-Qed.
-    
-Lemma interp_get_v_reduce: forall t hs s c f k bes,
-    const_exprs c bes ->
-    be_typing c bes (Tf [::] [::t]) ->
-    interp_get_v host_application_impl host_application_impl_correct hs s f bes = Some k ->
-    reduce_trans (hs, s, f, (to_e_list bes))
-                 (hs, s, f, [::$V k]).
-Proof.
-  move => t hs s c f k bes Hconst Hbet Heval.
-  eapply const_exprs_impl in Hconst; eauto.
-  destruct Hconst as [be [-> Hconst]].
-  unfold const_expr in Hconst.
-  destruct be => //.
-  1,2,3:
-    unfold interp_get_v in Heval;
-    simpl in Heval;
-    injection Heval as <-;
-    by constructor.
-  { (* ref_func *)
-    admit.
-  }
-  { (* global_get *) 
-    apply interp_get_v_sglob in Heval.
-    constructor.
-    unfold reduce_tuple.
-    by apply r_global_get.
-  }
-Admitted.
   
-Lemma interp_instantiate_imp_instantiate : forall hs s m v_imps s_end inst exps,
-  interp_instantiate host_application_impl host_application_impl_correct hs s m v_imps = Some (hs, s_end, inst, exps) ->
+Lemma interp_instantiate_imp_instantiate : forall hs hs' s m v_imps s_end inst exps,
+  interp_instantiate hs s m v_imps = Some (hs', s_end, inst, exps) ->
   instantiate s m v_imps (s_end, inst, exps).
 Proof.
-  move => hs s m v_imps s_end inst exps.
+  move => hs hs' s m v_imps s_end inst exps.
   unfold interp_instantiate, instantiate.
   move => Hinterp.
   destruct (module_type_checker m) as [[t_imps_mod t_exps] |] eqn:Hmodcheck => //.
   destruct (those _) as [t_imps | ] eqn:Hextcheck => //.
   destruct (all2 import_subtyping _ _) eqn:Hextsubtyping => //.
-  destruct (get_global_inits _ _ _ _ _ (mod_globals m)) as [g_inits |] eqn:Hglobinit => //.
-  destruct (get_elem_inits _ _ _ _ _ (mod_elems m)) as [r_inits |] eqn:Heleminit => //.
+  destruct (get_global_inits _ _ (mod_globals m)) as [g_inits |] eqn:Hglobinit => //.
+  destruct (get_elem_inits _ _ (mod_elems m)) as [r_inits |] eqn:Heleminit => //.
   destruct (interp_alloc_module s m v_imps g_inits r_inits) as [s' inst'] eqn:Halloc => //.
   injection Hinterp as <- <- Heq.
 
@@ -412,21 +288,13 @@ Proof.
   extract_premise.
 
   destruct s, s1, s2, s3, s4, s5, s6; simpl in *.
-(*
-  rewrite Hallocfuncs Halloctabs Hallocmems Hallocglobs Hallocelems Hallocdatas in Hallocmodule.
-  simpl in Hallocmodule; remove_bools_options.
-*)
   repeat split => //.
   - (* subtyping *)
     by eapply Forall2_all2_impl; eauto.
-(*  - (* store eq *)
-    repeat rewrite List.map_length.
-    by repeat rewrite eq_refl.*)
   - (* global initialisers -- hardest case, since it's the main difference in the 
        executable version *)
-    simpl.
     unfold instantiate_globals.
-    apply Forall2_spec; first by apply those_length in Hglobinit; rewrite length_is_size size_map in Hglobinit.
+    apply Forall2_spec => //.
     move => n mglob gv Hnth1 Hnth2.
     eapply those_map_lookup in Hglobinit as [gi [Hmap Hnth]]; last by eauto.
     apply module_typecheck_glob_aux in Hmodcheck as [C Hmodcheck].
@@ -436,89 +304,76 @@ Proof.
     move/andP in Hmodcheck.
     destruct Hmodcheck as [Hconstexpr Hbetype].
     move/b_e_type_checker_reflects_typing in Hbetype.
-    eapply interp_get_v_reduce; eauto.
     eapply const_exprs_impl in Hconstexpr; last by eauto.
     destruct Hconstexpr as [e [-> Hconst]].
     unfold const_expr in Hconst.
-    apply interp
-    destruct e => //.
+    destruct e => //; subst; simpl in Hmap.
     1,2,3: (* const_num/const_vec/ref_null *)
-      unfold interp_get_v in Hmap;
-      simpl in Hmap;
       injection Hmap as <-;
       simpl in *;
       simplify_multieq;
       by constructor.
     { (* ref_func *)
-      unfold interp_get_v in Hmap; simpl in Hmap.
-      
+      remove_bools_options; simplify_multieq.
+      by constructor; apply r_ref_func => /=.
     }
-    { (* get_global *)
-      move/andP in Hconst.
-      simpl in *.
-      destruct Hconst as [Hlen Himps].
-      destruct (ext_t_globs t_imps !! i) eqn:Himpslookup => //.
-      apply interp_get_v_sglob in Hglobinit.
-      constructor.
-      apply r_get_global => /=.
-      unfold sglob_val, sglob, sglob_ind in *.
-      simpl in *.
+    { (* global_get *)
+      remove_bools_options; simplify_multieq.
+      constructor; apply r_global_get => /=.
+      unfold sglob_val, sglob, sglob_ind in *; simpl in *.
       remove_bools_options.
-      rewrite List.nth_error_map in Hoption.
-      destruct ((ext_globs v_imps) !! i) as [[i0] | ] eqn:Hextv => //.
-      eapply vt_imps_globs_lookup in Hexttype; eauto; last by apply external_typing_relate.
-      destruct Hexttype as [n' [Hvimpslookup Htimpslookup]].
-      injection Halloc as <-<-<-.
-      simpl in *.
-      rewrite List.nth_error_map List.nth_error_app1; last by apply nth_error_Some_length in Hextv.
-      rewrite Hextv => /=.
-      rewrite List.nth_error_app1; last by apply nth_error_Some_length in Hoption.
-      by rewrite Hoption.
+      unfold lookup_N in *.
+      by erewrite nth_error_app_Some; eauto.
     }
-  - clear - instantiate Hmodcheck Helem.
-    unfold instantiate_elem.
-    apply Forall2_spec.
-    { apply those_length in Helem.
-      by rewrite length_is_size size_map -length_is_size in Helem.
-    }
-    move => n melem k Helemlookup Hoff.
-    eapply those_spec in Helem; eauto.
-    rewrite List.nth_error_map Helemlookup in Helem.
-    simpl in Helem.
-    injection Helem as Helem.
-    eapply module_typecheck_elem_aux in Hmodcheck.
-    destruct Hmodcheck as [c Helemcheck].
-    eapply all_projection in Helemcheck; eauto.
-    unfold module_elem_type_checker in Helemcheck.
-    destruct melem, modelem_table => /=.
-    remove_bools_options.
-    move/b_e_type_checker_reflects_typing in H2.
-    unfold interp_get_i32 in Helem; remove_bools_options.
-    destruct v => //; injection Helem as ->.
-    by eapply interp_get_v_reduce; eauto.
-  - clear - instantiate Hmodcheck Hdata.
-    unfold instantiate_data.
-    apply Forall2_spec.
-    { apply those_length in Hdata.
-      by rewrite length_is_size size_map -length_is_size in Hdata.
-    }
-    move => n mdata k Hdatalookup Hoff.
-    eapply those_spec in Hdata; eauto.
-    rewrite List.nth_error_map Hdatalookup in Hdata.
-    simpl in Hdata.
-    injection Hdata as Hdata.
-    eapply module_typecheck_data_aux in Hmodcheck.
-    destruct Hmodcheck as [c Hdatacheck].
-    eapply all_projection in Hdatacheck; eauto.
-    unfold module_data_type_checker in Hdatacheck.
-    destruct mdata, moddata_data => /=.
-    remove_bools_options.
-    move/b_e_type_checker_reflects_typing in H1.
-    unfold interp_get_i32 in Hdata; remove_bools_options.
-    destruct v => //; injection Hdata as ->.
-    by eapply interp_get_v_reduce; eauto.
-  - by unfold check_start.
+  - subst.
+    unfold instantiate_elems.
+    apply Forall2_spec => //.
+    move => n melem vs Hnth1 Hnth2.
+    eapply those_map_lookup in Heleminit as [ei [Hmap Hnth]]; last by eauto.
+    apply module_typecheck_elem_aux in Hmodcheck as [C Hmodcheck].
+    unfold module_elem_type_checker in Hmodcheck.
+    eapply all_projection in Hmodcheck; eauto.
+    destruct melem.
+    move/andP in Hmodcheck; destruct Hmodcheck as [Hmodcheck Hmode].
+    move/andP in Hmodcheck; destruct Hmodcheck as [Hconstexpr Hbetype].
+    simplify_multieq.
+    apply Forall2_spec => //=.
+    + apply those_length in Hmap.
+      by rewrite List.map_length in Hmap; simpl in Hmap.
+    + move => i bes vref Hnthinit Hnthei.
+      eapply all_projection in Hbetype; eauto.
+      eapply all_projection in Hconstexpr; eauto.
+      eapply those_map_lookup in Hmap as [vref' [Hmap Hnth']]; eauto.
+      move/b_e_type_checker_reflects_typing in Hbetype.
+      eapply const_exprs_impl in Hconstexpr; last by eauto.
+      destruct Hconstexpr as [e [-> Hconst]].
+      unfold const_expr in Hconst.
+      destruct e => //; subst; simpl in Hmap.
+      { (* ref_null *)
+        injection Hmap as <-.
+        simpl in *.
+        simplify_multieq.
+        by constructor.
+      }
+      { (* ref_func *)
+        remove_bools_options; simplify_multieq.
+        constructor => /=.
+        unfold interp_get_vref in Hmap.
+        simpl in Hmap; remove_bools_options.
+        by apply r_ref_func.
+      }
+      { (* global_get *)
+        unfold interp_get_vref in Hmap; simpl in Hmap.
+        remove_bools_options; simplify_multieq; destruct v => //.
+        injection Hmap as ->.
+        constructor.
+        replace (vref_to_e vref') with (v_to_e (VAL_ref vref')) => //.
+        eapply r_global_get => /=.
+        unfold sglob_val, sglob, sglob_ind in *; simpl in *.
+        remove_bools_options.
+        unfold lookup_N in *.
+        by erewrite nth_error_app_Some; eauto.
+      }
 Qed.
- *)
-Admitted.
+
 End Host.
